
Exprimer les vecteurs $\vec{u}$ et $\vec{v}$ Ã  l'aide des vecteurs $\overrightarrow{AB}$ et $\overrightarrow{AC}$.
\begin{enumerate}
\item $\vec{u}=2\overrightarrow{AB}-3\overrightarrow{CB}$

$\vec{u}=2\overrightarrow{AB}-3\left(\overrightarrow{CA}+\overrightarrow{AB}\right)$

$\vec{u}=2\overrightarrow{AB}-3\overrightarrow{CA}-3\overrightarrow{AB}$

$\vec{u}=-\overrightarrow{AB}+3\overrightarrow{AC}$



\item $\vec{v}=\frac{1}{2}\overrightarrow{BC}+ \frac{3}{4}\overrightarrow{AB}- \frac{1}{3}\overrightarrow{AC}$


$\vec{v}=\frac{1}{2}\overrightarrow{BA}+\frac{1}{2}\overrightarrow{AC}+ \frac{3}{4}\overrightarrow{AB}- \frac{1}{3}\overrightarrow{AC}$



$\vec{v}=-\frac{1}{2}\overrightarrow{AB}+\frac{1}{2}\overrightarrow{AC}+ \frac{3}{4}\overrightarrow{AB}- \frac{1}{3}\overrightarrow{AC}$


$\vec{v}=\frac{1}{4}\overrightarrow{AB}+\frac{1}{6}\overrightarrow{AC}$

\end{enumerate}