
Ã‰crire chaque somme de vecteurs sous la forme d'un seul vecteur.
\begin{enumerate}
\item $\overrightarrow{BC}-\overrightarrow{BA}+\overrightarrow{BD}-\overrightarrow{BC} =  \overrightarrow{BC}-\overrightarrow{BC}-\overrightarrow{BA}+\overrightarrow{BD} =  -\overrightarrow{BA}+\overrightarrow{BD} =  \overrightarrow{AB}+\overrightarrow{BC} = \overrightarrow{AC} $


\item $\overrightarrow{AB}+\overrightarrow{CD}- \left(\overrightarrow{AB}-\overrightarrow{BC} \right)= \overrightarrow{AB}+\overrightarrow{CD}- \overrightarrow{AB}+\overrightarrow{BC}=  \overrightarrow{AB}- \overrightarrow{AB}+\overrightarrow{CD} +\overrightarrow{BC} =  \overrightarrow{BC} + \overrightarrow{CD}= \overrightarrow{BD} $


\end{enumerate}